\int{\frac{ax^2+bx+c}{Ax^2+Bx+C}\,dx}=\begin{cases}\frac{a}{3C}x^3+\frac{b}{2C}x^2+\frac{c}{C}x,&\text{when }A=0,B=0,C\neq0\\\frac{b}{B}x+\frac{Bc-Cb}{B^2}\ln\left|Bx+C\right|&\text{when }A=0,B\neq0,a=0\\\frac{a}{2B}x^2+\frac{Bab-Ca^2}{B^2a}x+\frac{B^2c-BCb+C^2a}{B^3}\ln\left|Bx+C\right|&\text{when }A=0,B\neq0,a\neq0\\\frac{a}{A}x+\frac{Ab-Ba}{2A^2}\ln\left|Ax^2+Bx+C\right|+\frac{2A^2c-ABb-2ACa+B^2a}{A^2\sqrt{4AC-B^2}}\tan^{-1}{\frac{2Ax+B}{\sqrt{4AC-B^2}}}&\text{when }A\neq0,B^2-4AC<0\\\frac{a}{A}x+\frac{Ab-Ba}{A^2}\ln\left|2Ax+B\right|+\frac{-2A^2c+ABb+2ACa-B^2a}{A^2\left(2Ax+B\right)}&\text{when }A\neq0,B^2-4AC=0\\\frac{a}{A}x+\frac{Ab-Ba}{2A^2}\ln\left|Ax^2+Bx+C\right|+\frac{2A^2c-ABb-2ACa+B^2a}{A^2\sqrt{B^2-4AC}}\ln\left|\frac{2Ax+B-\sqrt{B^2-4AC}}{\sqrt{\left|Ax^2+Bx+C\right|}}\right|&\text{when }A\neq0,B^2-4AC>0\end{cases}
